theories/Inductives.v
@@ -45,9 +45,7 @@ Arguments catchE {_ _}.
 Definition catchMap := @catchMap max_steps _ TimeoutErr. 
 Arguments catchMap {_ _}. 
   
-Instance trace_monad : Monad (@TraceM guard_exc).
-apply trace_monad. exact max_steps. exact TimeoutErr.
-Defined.
+Instance: Monad (@TraceM guard_exc) := @trace_monad max_steps guard_exc.
 
 (* Notation "'exc' A" := (excOn guard_exc A) (at level 100) : exc_scope.  *)
 Notation "'exc' A" := (@TraceM guard_exc A) (at level 100) : exc_scope. 
@@ -55,7 +53,7 @@ Notation "'exc' A" := (@TraceM guard_exc A) (at level 100) : exc_scope.
 Definition unwrap := @trc_unwrap.
 Arguments unwrap { _ _ _ _}. 
 
-Instance: TrcUnwrap list := @list_trc_unwrap max_steps _ TimeoutErr.
+Instance: TrcUnwrap list := @list_trc_unwrap max_steps guard_exc.
 
 Notation "a == b" := (eqb a b) (at level 70) : exc_scope. 
 Notation "a != b" := (negb(a==b)) (at level 90) : exc_scope.
